Orderedtree/DOrderedTree/Internal/Lemmas.lean
@@ -18,9 +18,9 @@ open Std.DHashMap.Internal.List
 
 universe u v
 
-variable {α : Type u} {β : α → Type v}
-
 namespace Std.DOrderedTree.Internal.Impl
+
+variable {α : Type u} {β : α → Type v} {_ : Ord α} {t : Impl α β}
 
 /-- Internal implementation detail of the hash map -/
 scoped macro "wf_trivial" : tactic => `(tactic|
@@ -52,20 +52,18 @@ scoped syntax "simp_to_model" ("using" term)? : tactic
 
 macro_rules
 | `(tactic| simp_to_model $[using $using?]?) => do
-  let mut congrModify : Array (TSyntax `term) := #[]
-  for congr in (← congrNames) do
-    for modify in modifyNames do
-      congrModify := congrModify.push (← `($congr:term ($(mkIdent modify) ..)))
-  `(tactic|
-    (simp (discharger := wf_trivial) only
-      [$[$(Array.map Lean.mkIdent queryNames):term],*, $[$congrModify:term],*]
-     $[apply $(using?.toArray):term];*)
-    <;> wf_trivial)
+    let mut congrModify : Array (TSyntax `term) := #[]
+    for congr in (← congrNames) do
+      for modify in modifyNames do
+        congrModify := congrModify.push (← `($congr:term ($(mkIdent modify) ..)))
+    `(tactic|
+      (simp (discharger := wf_trivial) only
+        [$[$(Array.map Lean.mkIdent queryNames):term],*, $[$congrModify:term],*]
+       $[apply $(using?.toArray):term];*)
+      <;> wf_trivial)
 
 attribute [local instance] beqOfOrd
 attribute [local instance] equivBEq_of_transOrd
-
-variable {_ : Ord α} {t : Impl α β}
 
 theorem isEmpty_empty : isEmpty (empty : Impl α β) := by
   simp [Impl.isEmpty_eq_isEmpty]
@@ -73,25 +71,32 @@ theorem isEmpty_empty : isEmpty (empty : Impl α β) := by
 theorem mem_iff_contains {k : α} : k ∈ t ↔ t.contains k :=
   Iff.rfl
 
-theorem contains_congr {k k' : α} (hab : compare k k' = .eq) :
-    t.contains k = t.contains k' :=
-  sorry
+theorem contains_congr [TransOrd α] (h : t.WF) {k k' : α} (hab : k == k') :
+    t.contains k = t.contains k' := by
+  simp_to_model using List.containsKey_congr
 
-theorem mem_congr {k k' : α} (hab : compare k k' = .eq) : k ∈ t ↔ k' ∈ t := by
-  simp [mem_iff_contains, contains_congr hab]
+theorem mem_congr [TransOrd α] (h : t.WF) {k k' : α} (hab : k == k') : k ∈ t ↔ k' ∈ t := by
+  simp [mem_iff_contains, contains_congr h hab]
 
-theorem contains_empty {k : α} : (empty : Impl α β).contains k = false :=
-  sorry
+theorem contains_empty {k : α} : (empty : Impl α β).contains k = false := by
+  simp [contains]
 
-theorem mem_empty {k : α} : k ∉ (empty : Impl α β) :=
- sorry
+theorem mem_empty {k : α} : k ∉ (empty : Impl α β) := by
+  simp [mem_iff_contains, contains_empty]
 
-theorem contains_insert [TransOrd α] (t : Impl α β) (h : t.WF) {k a : α} {v : β k} :
+theorem contains_insert [TransOrd α] (h : t.WF) {k a : α} {v : β k} :
     (t.insert k v h.balanced).impl.contains a = (compare k a == .eq || t.contains a) := by
   simp_to_model using List.containsKey_insertEntry
 
-theorem contains_insertSlow [TransOrd α] (t : Impl α β) (h : t.WF) {k a : α} {v : β k} :
+theorem contains_insertSlow [TransOrd α] (h : t.WF) {k a : α} {v : β k} :
     (t.insertSlow k v).contains a = (compare k a == .eq || t.contains a) := by
   simp_to_model using List.containsKey_insertEntry
 
 end Std.DOrderedTree.Internal.Impl
+
+/-- Used as instance by the dependents of this file -/
+theorem TransOrd.ofTransCmp {α : Type u} {cmp : α → α → Ordering} [TransCmp cmp] :
+    letI _ : Ord α := ⟨cmp⟩; TransOrd α :=
+  let _ : Ord α := ⟨cmp⟩
+  have _ : OrientedOrd α := ⟨⟩
+  ⟨TransCmp.le_trans⟩
