Orderedtree/OrderedSet/Lemmas.lean
@@ -17,15 +17,31 @@ open Std.DOrderedTree.Internal
 
 universe u v
 
-variable {α : Type u} {cmp : α → α → Ordering}
-
 namespace Std.OrderedSet
+
+variable {α : Type u} {cmp : α → α → Ordering} {t : OrderedSet α cmp}
 
 theorem isEmpty_empty : (empty : OrderedSet α cmp).isEmpty :=
   OrderedTree.isEmpty_empty
 
-theorem contains_insert [h : TransCmp cmp] (m : OrderedSet α cmp) {k a : α} :
-    (m.insert k).contains a = (cmp k a == .eq || m.contains a) :=
-  OrderedTree.contains_insert m.inner
+theorem mem_iff_contains {k : α} : k ∈ t ↔ t.contains k :=
+  OrderedTree.mem_iff_contains
+
+theorem contains_congr [TransCmp cmp] {k k' : α} (hab : cmp k k' == .eq) :
+    t.contains k = t.contains k' :=
+  OrderedTree.contains_congr hab
+
+theorem mem_congr [TransCmp cmp] {k k' : α} (hab : cmp k k' == .eq) : k ∈ t ↔ k' ∈ t :=
+  OrderedTree.mem_congr hab
+
+theorem contains_empty {k : α} : (empty : OrderedSet α cmp).contains k = false :=
+  OrderedTree.contains_empty
+
+theorem mem_empty {k : α} : k ∉ (empty : OrderedSet α cmp) :=
+  OrderedTree.mem_empty
+
+theorem contains_insert [h : TransCmp cmp] (t : OrderedSet α cmp) {k a : α} :
+    (t.insert k).contains a = (cmp k a == .eq || t.contains a) :=
+  OrderedTree.contains_insert
 
 end Std.OrderedSet
